proof/invariants/InitFstShadow.v
@@ -300,9 +300,9 @@ Qed.
 
 Lemma initFstShadowPrepareHT lpred ptMMUTrdVA phySh2addr phySh1addr indMMUToPrepare ptMMUFstVA phyMMUaddr
       lastLLTable phyPDChild currentShadow2 phySh2Child currentPD ptSh1TrdVA ptMMUSndVA ptSh1SndVA ptSh1FstVA
-      currentShadow1 descChildphy phySh1Child currentPart trdVA nextVA vaToPrepare sndVA fstVA nbLgen l  idxFstVA idxSndVA idxTrdVA zeroI LLroot LLChildphy newLastLLable minFI:
+      currentShadow1 descChildphy phySh1Child currentPart trdVA nextVA vaToPrepare sndVA fstVA nbLgen l  idxFstVA idxSndVA idxTrdVA zeroI LLroot LLChildphy newLastLLable minFI indMMUToPreparebool:
 {{ fun s : state =>
-(propagatedPropertiesPrepare LLroot LLChildphy newLastLLable s ptMMUTrdVA phySh2addr phySh1addr indMMUToPrepare ptMMUFstVA phyMMUaddr
+(propagatedPropertiesPrepare indMMUToPreparebool LLroot LLChildphy newLastLLable s ptMMUTrdVA phySh2addr phySh1addr indMMUToPrepare ptMMUFstVA phyMMUaddr
   lastLLTable phyPDChild currentShadow2 phySh2Child currentPD ptSh1TrdVA ptMMUSndVA ptSh1SndVA ptSh1FstVA
   currentShadow1 descChildphy phySh1Child currentPart trdVA nextVA vaToPrepare sndVA fstVA nbLgen l false
   false false true true true idxFstVA idxSndVA idxTrdVA zeroI minFI
@@ -312,7 +312,7 @@ Lemma initFstShadowPrepareHT lpred ptMMUTrdVA phySh2addr phySh1addr indMMUToPrep
 /\ writeAccessibleRecPreparePostcondition currentPart phySh2addr s 
 /\ StateLib.Level.pred l = Some lpred) 
 /\ isWellFormedMMUTables phyMMUaddr s }} initFstShadow phySh1addr lpred zeroI 
-{{fun _ s => (propagatedPropertiesPrepare LLroot LLChildphy newLastLLable s ptMMUTrdVA phySh2addr phySh1addr indMMUToPrepare ptMMUFstVA phyMMUaddr
+{{fun _ s => (propagatedPropertiesPrepare indMMUToPreparebool LLroot LLChildphy newLastLLable s ptMMUTrdVA phySh2addr phySh1addr indMMUToPrepare ptMMUFstVA phyMMUaddr
   lastLLTable phyPDChild currentShadow2 phySh2Child currentPD ptSh1TrdVA ptMMUSndVA ptSh1SndVA ptSh1FstVA
   currentShadow1 descChildphy phySh1Child currentPart trdVA nextVA vaToPrepare sndVA fstVA nbLgen l false
   false false true true true idxFstVA idxSndVA idxTrdVA zeroI minFI
