proof/invariants/UpdateShadow1StructurePrepare.v
@@ -49,17 +49,17 @@ Lemma propagatedPropertiesPrepareUpdateShadow1Structure b1 b2 b3 b4 b5 b6  (vaVa
        ptMMUTrdVA phySh2addr phySh1addr indMMUToPrepare
        ptMMUFstVA phyMMUaddr lastLLTable phyPDChild currentShadow2 phySh2Child currentPD
        ptSh1TrdVA ptMMUSndVA ptSh1SndVA ptSh1FstVA currentShadow1 descChildphy phySh1Child
-       currentPart trdVA nextVA vaToPrepare sndVA fstVA nbLgen l idxFstVA idxSndVA idxTrdVA zeroI LLroot LLChildphy newLastLLable minFI:
+       currentPart trdVA nextVA vaToPrepare sndVA fstVA nbLgen l idxFstVA idxSndVA idxTrdVA zeroI LLroot LLChildphy newLastLLable minFI indMMUToPreparebool:
 PCToGeneralizePropagatedPropertiesPrepareUpdateShadow1Structure b1 b2 b3 b4 b5 b6  
 vaValue fstVA sndVA trdVA ptMMU ptSh1 pg ptSh1FstVA ptSh1SndVA ptSh1TrdVA phyMMUaddr phySh1addr phySh2addr
  ptMMUFstVA ptMMUSndVA ptMMUTrdVA idxFstVA idxSndVA idxTrdVA idx-> 
 isPartitionFalse ptSh1 idx s ->
-propagatedPropertiesPrepare LLroot LLChildphy newLastLLable s ptMMUTrdVA phySh2addr phySh1addr indMMUToPrepare
+propagatedPropertiesPrepare indMMUToPreparebool LLroot LLChildphy newLastLLable s ptMMUTrdVA phySh2addr phySh1addr indMMUToPrepare
        ptMMUFstVA phyMMUaddr lastLLTable phyPDChild currentShadow2 phySh2Child currentPD
        ptSh1TrdVA ptMMUSndVA ptSh1SndVA ptSh1FstVA currentShadow1 descChildphy phySh1Child
        currentPart trdVA nextVA vaToPrepare sndVA fstVA nbLgen l false false false b1 b2 b3
         idxFstVA idxSndVA idxTrdVA zeroI minFI -> 
-propagatedPropertiesPrepare LLroot LLChildphy newLastLLable {|  currentPartition := currentPartition s;
+propagatedPropertiesPrepare indMMUToPreparebool LLroot LLChildphy newLastLLable {|  currentPartition := currentPartition s;
                                  memory := add ptSh1 idx (VE {| pd := false; va := vaValue |}) (memory s) beqPage beqIndex |}
        ptMMUTrdVA phySh2addr phySh1addr indMMUToPrepare
        ptMMUFstVA phyMMUaddr lastLLTable phyPDChild currentShadow2 phySh2Child currentPD
@@ -253,9 +253,9 @@ Admitted.
 
 Lemma writeVirEntryFstVA ptMMUTrdVA phySh2addr phySh1addr indMMUToPrepare ptMMUFstVA phyMMUaddr lastLLTable phyPDChild
       currentShadow2 phySh2Child currentPD ptSh1TrdVA ptMMUSndVA ptSh1SndVA ptSh1FstVA currentShadow1 descChildphy phySh1Child
-      currentPart trdVA nextVA vaToPrepare sndVA fstVA nbLgen l idxFstVA idxSndVA idxTrdVA zeroI lpred LLroot LLChildphy newLastLLable minFI:
+      currentPart trdVA nextVA vaToPrepare sndVA fstVA nbLgen l idxFstVA idxSndVA idxTrdVA zeroI lpred LLroot LLChildphy newLastLLable minFI indMMUToPreparebool:
 {{ fun s : state =>
-   propagatedPropertiesPrepare LLroot LLChildphy newLastLLable s ptMMUTrdVA phySh2addr phySh1addr indMMUToPrepare ptMMUFstVA phyMMUaddr lastLLTable phyPDChild
+   propagatedPropertiesPrepare indMMUToPreparebool LLroot LLChildphy newLastLLable s ptMMUTrdVA phySh2addr phySh1addr indMMUToPrepare ptMMUFstVA phyMMUaddr lastLLTable phyPDChild
       currentShadow2 phySh2Child currentPD ptSh1TrdVA ptMMUSndVA ptSh1SndVA ptSh1FstVA currentShadow1 descChildphy phySh1Child
       currentPart trdVA nextVA vaToPrepare sndVA fstVA nbLgen l false false false true true true idxFstVA idxSndVA idxTrdVA zeroI minFI
    /\ isPartitionFalseAll s ptSh1FstVA ptSh1TrdVA ptSh1SndVA idxFstVA idxSndVA idxTrdVA 
@@ -266,7 +266,7 @@ Lemma writeVirEntryFstVA ptMMUTrdVA phySh2addr phySh1addr indMMUToPrepare ptMMUF
   writeVirEntry ptSh1FstVA idxFstVA fstVA 
   
   {{fun _ s  => 
-   propagatedPropertiesPrepare LLroot LLChildphy newLastLLable s ptMMUTrdVA phySh2addr phySh1addr indMMUToPrepare ptMMUFstVA phyMMUaddr lastLLTable phyPDChild
+   propagatedPropertiesPrepare indMMUToPreparebool LLroot LLChildphy newLastLLable s ptMMUTrdVA phySh2addr phySh1addr indMMUToPrepare ptMMUFstVA phyMMUaddr lastLLTable phyPDChild
       currentShadow2 phySh2Child currentPD ptSh1TrdVA ptMMUSndVA ptSh1SndVA ptSh1FstVA currentShadow1 descChildphy phySh1Child
       currentPart trdVA nextVA vaToPrepare sndVA fstVA nbLgen l false false false false true true idxFstVA idxSndVA idxTrdVA zeroI minFI
    /\ isPartitionFalse ptSh1SndVA idxSndVA s 
@@ -322,9 +322,9 @@ Qed.
 
 Lemma writeVirEntrySndVA ptMMUTrdVA phySh2addr phySh1addr indMMUToPrepare ptMMUFstVA phyMMUaddr lastLLTable phyPDChild
       currentShadow2 phySh2Child currentPD ptSh1TrdVA ptMMUSndVA ptSh1SndVA ptSh1FstVA currentShadow1 descChildphy phySh1Child
-      currentPart trdVA nextVA vaToPrepare sndVA fstVA nbLgen l idxFstVA idxSndVA idxTrdVA zeroI lpred LLroot LLChildphy newLastLLable minFI:
+      currentPart trdVA nextVA vaToPrepare sndVA fstVA nbLgen l idxFstVA idxSndVA idxTrdVA zeroI lpred LLroot LLChildphy newLastLLable minFI indMMUToPreparebool:
 {{ fun s : state =>
-   propagatedPropertiesPrepare LLroot LLChildphy newLastLLable s ptMMUTrdVA phySh2addr phySh1addr indMMUToPrepare ptMMUFstVA
+   propagatedPropertiesPrepare indMMUToPreparebool LLroot LLChildphy newLastLLable s ptMMUTrdVA phySh2addr phySh1addr indMMUToPrepare ptMMUFstVA
      phyMMUaddr lastLLTable phyPDChild currentShadow2 phySh2Child currentPD ptSh1TrdVA
      ptMMUSndVA ptSh1SndVA ptSh1FstVA currentShadow1 descChildphy phySh1Child currentPart
      trdVA nextVA vaToPrepare sndVA fstVA nbLgen l false false false false true true idxFstVA
@@ -337,7 +337,7 @@ Lemma writeVirEntrySndVA ptMMUTrdVA phySh2addr phySh1addr indMMUToPrepare ptMMUF
   writeVirEntry ptSh1SndVA idxSndVA sndVA 
     
   {{fun _ s  => 
-   propagatedPropertiesPrepare LLroot LLChildphy newLastLLable s ptMMUTrdVA phySh2addr phySh1addr indMMUToPrepare ptMMUFstVA phyMMUaddr lastLLTable phyPDChild
+   propagatedPropertiesPrepare indMMUToPreparebool LLroot LLChildphy newLastLLable s ptMMUTrdVA phySh2addr phySh1addr indMMUToPrepare ptMMUFstVA phyMMUaddr lastLLTable phyPDChild
       currentShadow2 phySh2Child currentPD ptSh1TrdVA ptMMUSndVA ptSh1SndVA ptSh1FstVA currentShadow1 descChildphy phySh1Child
       currentPart trdVA nextVA vaToPrepare sndVA fstVA nbLgen l false false false false false true idxFstVA idxSndVA idxTrdVA zeroI minFI
    /\ isPartitionFalse ptSh1TrdVA idxTrdVA s
@@ -402,9 +402,9 @@ Qed.
  
 Lemma writeVirEntryTrdVA ptMMUTrdVA phySh2addr phySh1addr indMMUToPrepare ptMMUFstVA phyMMUaddr lastLLTable phyPDChild
       currentShadow2 phySh2Child currentPD ptSh1TrdVA ptMMUSndVA ptSh1SndVA ptSh1FstVA currentShadow1 descChildphy phySh1Child
-      currentPart trdVA nextVA vaToPrepare sndVA fstVA nbLgen l idxFstVA idxSndVA idxTrdVA zeroI lpred LLroot LLChildphy newLastLLable minFI:
+      currentPart trdVA nextVA vaToPrepare sndVA fstVA nbLgen l idxFstVA idxSndVA idxTrdVA zeroI lpred LLroot LLChildphy newLastLLable minFI indMMUToPreparebool:
 {{ fun s : state =>
-   propagatedPropertiesPrepare LLroot LLChildphy newLastLLable s ptMMUTrdVA phySh2addr phySh1addr indMMUToPrepare ptMMUFstVA
+   propagatedPropertiesPrepare indMMUToPreparebool LLroot LLChildphy newLastLLable s ptMMUTrdVA phySh2addr phySh1addr indMMUToPrepare ptMMUFstVA
      phyMMUaddr lastLLTable phyPDChild currentShadow2 phySh2Child currentPD ptSh1TrdVA
      ptMMUSndVA ptSh1SndVA ptSh1FstVA currentShadow1 descChildphy phySh1Child currentPart
      trdVA nextVA vaToPrepare sndVA fstVA nbLgen l false false false false false true idxFstVA
@@ -418,7 +418,7 @@ Lemma writeVirEntryTrdVA ptMMUTrdVA phySh2addr phySh1addr indMMUToPrepare ptMMUF
   writeVirEntry ptSh1TrdVA idxTrdVA trdVA 
     
   {{fun _ s  => 
-   propagatedPropertiesPrepare LLroot LLChildphy newLastLLable s ptMMUTrdVA phySh2addr phySh1addr indMMUToPrepare ptMMUFstVA phyMMUaddr lastLLTable phyPDChild
+   propagatedPropertiesPrepare indMMUToPreparebool LLroot LLChildphy newLastLLable s ptMMUTrdVA phySh2addr phySh1addr indMMUToPrepare ptMMUFstVA phyMMUaddr lastLLTable phyPDChild
       currentShadow2 phySh2Child currentPD ptSh1TrdVA ptMMUSndVA ptSh1SndVA ptSh1FstVA currentShadow1 descChildphy phySh1Child
       currentPart trdVA nextVA vaToPrepare sndVA fstVA nbLgen l false false false false false false idxFstVA idxSndVA idxTrdVA zeroI minFI
    /\ writeAccessibleRecPreparePostconditionAll currentPart phyMMUaddr phySh1addr phySh2addr s 
