proof/invariants/WriteIndex.v
@@ -2659,13 +2659,13 @@ Qed.
 Lemma insertEntryIntoLLPCUpdateLLIndex s ptMMUTrdVA phySh2addr phySh1addr indMMUToPrepare ptMMUFstVA phyMMUaddr lastLLTable
       phyPDChild currentShadow2 phySh2Child currentPD ptSh1TrdVA ptMMUSndVA ptSh1SndVA ptSh1FstVA currentShadow1
       descChildphy phySh1Child currentPart trdVA nextVA vaToPrepare sndVA fstVA nbLgen l idxFstVA idxSndVA idxTrdVA
-      zeroI lpred newLastLLable  (* (LLDescChild:page) *) entry fstLL LLChildphy  newFFI (minFI minFI' idx:index):
+      zeroI lpred newLastLLable  (* (LLDescChild:page) *) entry fstLL LLChildphy  newFFI (minFI minFI' idx:index) indMMUToPreparebool:
 lookup newLastLLable idx (memory s) beqPage beqIndex = Some (I entry) ->
 (* StateLib.getMaxIndex <> Some nextFFI ->   *)
 insertEntryIntoLLPC s ptMMUTrdVA phySh2addr phySh1addr indMMUToPrepare ptMMUFstVA phyMMUaddr lastLLTable
       phyPDChild currentShadow2 phySh2Child currentPD ptSh1TrdVA ptMMUSndVA ptSh1SndVA ptSh1FstVA currentShadow1
       descChildphy phySh1Child currentPart trdVA nextVA vaToPrepare sndVA fstVA nbLgen l idxFstVA idxSndVA idxTrdVA
-      zeroI lpred fstLL LLChildphy newLastLLable minFI->
+      zeroI lpred fstLL LLChildphy newLastLLable minFI indMMUToPreparebool->
 (exists NbFI : index, isIndexValue newLastLLable (CIndex 1) NbFI {|
   currentPartition := currentPartition s;
   memory := add newLastLLable idx (I newFFI) (memory s) beqPage beqIndex |} /\ NbFI >= minFI') ->
@@ -2674,7 +2674,7 @@ insertEntryIntoLLPC {|
   memory := add newLastLLable idx (I newFFI) (memory s) beqPage beqIndex |} ptMMUTrdVA phySh2addr phySh1addr indMMUToPrepare ptMMUFstVA phyMMUaddr lastLLTable
       phyPDChild currentShadow2 phySh2Child currentPD ptSh1TrdVA ptMMUSndVA ptSh1SndVA ptSh1FstVA currentShadow1
       descChildphy phySh1Child currentPart trdVA nextVA vaToPrepare sndVA fstVA nbLgen l idxFstVA idxSndVA idxTrdVA
-      zeroI lpred fstLL LLChildphy newLastLLable minFI'.
+      zeroI lpred fstLL LLChildphy newLastLLable minFI' indMMUToPreparebool.
 Proof.
 intros Hlookup (* Hkey2 *).
 intros.
