proof/invariants/writePhysical.v
@@ -2676,7 +2676,7 @@ Qed.
 Lemma insertEntryIntoLLPCUpdateLLCouplePPVA s ptMMUTrdVA phySh2addr phySh1addr indMMUToPrepare ptMMUFstVA phyMMUaddr lastLLTable
       phyPDChild currentShadow2 phySh2Child currentPD ptSh1TrdVA ptMMUSndVA ptSh1SndVA ptSh1FstVA currentShadow1
       descChildphy phySh1Child currentPart trdVA nextVA vaToPrepare sndVA fstVA nbLgen l idxFstVA idxSndVA idxTrdVA
-      zeroI lpred newLastLLable nextFFI (* (LLDescChild:page) *) entry fstLL LLChildphy minFI:
+      zeroI lpred newLastLLable nextFFI (* (LLDescChild:page) *) entry fstLL LLChildphy minFI indMMUToPreparebool:
 lookup newLastLLable nextFFI (memory s) beqPage beqIndex = Some (PP entry) ->
 StateLib.getMaxIndex <> Some nextFFI ->  
 insertEntryIntoLLPC s ptMMUTrdVA phySh2addr phySh1addr indMMUToPrepare ptMMUFstVA phyMMUaddr lastLLTable
